Forbid 2 and 4-bit kinds

src/Dafny/jrnl/kinds.s.dfy
@@ -9,12 +9,14 @@ import opened Pow
 // but expressing that a kind is a power of two would be complicated, so we
 // define them as the power of two. This is easier to work with but annoying to
 // construct.
-type Kind = k:int | 0 <= k <= 15
+type Kind = k:int | 0 == k || 3 <= k <= 15
 
+const KindBit: Kind := 0
 const KindByte: Kind := 3
 const KindUInt64: Kind := KindByte + 3
 const KindInode: Kind := KindByte + 7 // 2^7 = 128 bytes
 
+// kindSize interprets a kind as a size in bits
 function method kindSize(k: Kind): (sz:nat)
 ensures sz > 0
 {
@@ -54,6 +56,20 @@ requires k >= 3
 ensures kindSize(k)/8*8 == kindSize(k)
 {
     kind_at_least_byte_iff(k);
+}
+
+lemma kind_size_cases(k: Kind)
+ensures (&& k == 0
+         && kindSize(k)==1) ||
+        (&& k >= 3
+         && kindSize(k) >= 8
+         && kindSize(k) % 8 == 0)
+{
+    if k >= 3 {
+        assert pow(2, 3) == 8;
+        pow_increasing(2, k, 3);
+        pow_plus(2, k, k-3);
+    }
 }
 
 }
